generational/spec/GC.Gen.CheneyPreservation.fsti
@@ -507,6 +507,30 @@ val chunked_cheney_forward_one_head_split_preserves_chunked_alloc_shape
          SpecMajorAlloc.major_fl_chain_terminates
           cs'.ccs_major cs'.ccs_fp fuel = true))
 
+val chunked_cheney_forward_one_budget_ready
+  : minor:minor_state -> cs:ChunkedCheney.chunked_cheney_state ->
+    addr:U64.t -> remaining:nat -> GTot prop
+
+val chunked_cheney_forward_one_head_split_preserves_remaining_head_wosize
+  : minor:minor_state -> cs:ChunkedCheney.chunked_cheney_state ->
+    addr:U64.t -> fuel:nat -> remaining:nat ->
+    Lemma
+      (requires
+        fuel > 1 /\
+        GenInv.chunked_major_alloc_shape cs.ccs_major cs.ccs_fp fuel /\
+        SpecMajorAlloc.major_fl_chain_terminates
+          cs.ccs_major cs.ccs_fp fuel = true /\
+        chunked_cheney_forward_one_budget_ready
+          minor cs addr remaining)
+      (ensures
+        (let cs' =
+          ChunkedCheney.chunked_cheney_forward_one minor cs addr fuel in
+         GenInv.chunked_major_alloc_shape cs'.ccs_major cs'.ccs_fp fuel /\
+         SpecMajorAlloc.major_fl_chain_terminates
+          cs'.ccs_major cs'.ccs_fp fuel = true /\
+         SpecMajorAlloc.major_fl_head_wosize
+          cs'.ccs_major cs'.ccs_fp >= remaining))
+
 val chunked_cheney_forward_one_split_ready
   : minor:minor_state -> cs:ChunkedCheney.chunked_cheney_state ->
     addr:U64.t -> GTot prop
